sepcomp/seq_lemmas.v
@@ -1,0 +1,82 @@
+Require Import ssreflect ssrbool ssrnat ssrfun eqtype seq.
+Set Implicit Arguments.
+Unset Strict Implicit.
+Unset Printing Implicit Defensive.
+
+Fixpoint All T P (l : seq T) :=
+  match l with
+    | nil => True
+    | a :: l' => [/\ P a & All P l']
+  end.
+
+Fixpoint All2_aux T P (a : T) (l : seq T) :=
+  if l is [:: a' & l'] then
+    [/\ P a a' & All2_aux P a l']
+  else True. 
+
+Fixpoint All2 T (P : T -> T -> Prop) (l : seq T) :=
+  if l is [:: a & l'] then [/\ All2_aux P a l' & All2 P l']
+  else True.
+
+Lemma All2_cons T P (a : T) (l : seq T) :
+  All2 P [:: a & l] <-> [/\ All2_aux P a l & All2 P l].
+Proof. by split=> /= => [][]A B; split. Qed.
+
+Lemma All2_aux_sub T (P P' : T -> T -> Prop) a l :
+  All2_aux P a l -> (forall a a', P a a' -> P' a a') -> All2_aux P' a l.
+Proof.
+move=> A B; move: A; elim: l=> // a' l' IH /= []C D; split.
+by apply: (B _ _ C).
+by apply: IH.
+Qed.
+
+Lemma All2_sub T (P P' : T -> T -> Prop) l :
+  All2 P l -> (forall a a', P a a' -> P' a a') -> All2 P' l.
+Proof.
+move=> A B; move: A; elim: l=> // a l' IH /= []C D; split.
+by apply: (All2_aux_sub C).
+by apply: (IH D).
+Qed.
+
+Lemma All2C T (P : T -> T -> Prop) a b l :
+  All2 P (a :: b :: l) -> 
+  (forall a b, P a b -> P b a) -> 
+  All2 P (b :: a :: l).
+Proof.
+move=> /= => [][][]A B []C D HC; split=> //.
+by split=> //; apply: (HC _ _ A).
+Qed.
+
+Lemma All2_aux_comp T U (P : T -> T -> Prop) (f : U -> T) a l :
+  All2_aux (fun a b : U => P (f a) (f b)) a l <-> 
+  All2_aux P (f a) (map f l).
+Proof.
+move: a; elim: l=> // a' l' IH a''; split.
+by move=> /= []A B; split=> //; rewrite -IH.
+by move=> /= []A B; split=> //; rewrite IH.
+Qed.
+
+Lemma All2_comp T U (P : T -> T -> Prop) (f : U -> T) l :
+  All2 (fun a b => P (f a) (f b)) l <-> 
+  (All2 P \o map f) l.
+Proof.
+elim: l=> // a l' IH; split.
+move=> /= []A B; split; first by rewrite -All2_aux_comp. 
+by case: IH; move/(_ B)=> C _; apply: C.
+move=> /= []A B; split; first by rewrite All2_aux_comp.
+by case: IH=> _; move/(_ B).
+Qed.
+
+Lemma All2_comp' T U (P : T -> T -> Prop) (f : U -> T) l :
+  All2 (fun a b => P (f a) (f b)) l <-> 
+  All2 P (map f l).
+Proof.
+cut (All2 (fun a b => P (f a) (f b)) l <-> 
+    (All2 P \o map f) l).
+by move=> ->.
+by apply: All2_comp.
+Qed.
+
+
+
+
